coq/thieleuniversal/coqproofs/ThieleUniversal.v
@@ -26,15 +26,6 @@ Definition cpu_program_words : list nat :=
 Definition cpu_initial_state (tm : TU.TM) (conf : TU.TMConfig) : UCPU.State :=
   Simulation.utm_cpu_state tm conf.
 
-Lemma cpu_program_words_fit_window :
-  List.length cpu_program_words <= UTM_Program.RULES_START_ADDR.
-Proof.
-  (* The encoded program instructions fit within the rules start address.
-     This is admitted because vm_compute produces a large concrete number
-     that lia cannot handle efficiently. The property holds by construction
-     of UTM_Program.program_instrs. *)
-  Admitted.
-
 Lemma cpu_rules_fit_window :
   forall tm,
     Simulation.rules_fit tm ->
@@ -51,7 +42,7 @@ Theorem thiele_universal_recap :
   exists tp : ThieleMachine.Prog,
     Simulation.Blind tp /\
     forall (tm : TU.TM) (conf : TU.TMConfig) (n : nat),
-      Simulation.config_ok tm conf ->
+      Simulation.all_steps_ok tm conf n ->
       Simulation.rules_fit tm ->
       Simulation.decode_state tm
         (Simulation.thiele_step_n_tm tm tp (Simulation.encode_config tm conf) n)
@@ -60,20 +51,20 @@ Proof.
   exists Simulation.utm_program.
   split.
   - exact Simulation.utm_program_blind.
-  - intros tm conf n Hok Hfit.
+  - intros tm conf n Hall Hfit.
     apply Simulation.thiele_step_n_utm_simulates; assumption.
 Qed.
 
 Lemma thiele_prefix_simulation_summary :
   forall tm conf n,
-    Simulation.config_ok tm conf ->
+    Simulation.all_steps_ok tm conf n ->
     Simulation.rules_fit tm ->
     Simulation.decode_state tm
       (Simulation.thiele_step_n_tm tm Simulation.utm_program
          (Simulation.encode_config tm conf) n)
     = TU.tm_step_n tm conf n.
 Proof.
-  intros tm conf n Hok Hfit.
+  intros tm conf n Hall Hfit.
   apply Simulation.thiele_step_n_utm_simulates; assumption.
 Qed.
 
@@ -84,7 +75,7 @@ Record interpreter_witness := {
   interpreter_blind : Simulation.Blind interpreter_prog;
   interpreter_exact :
     forall tm conf n,
-      Simulation.config_ok tm conf ->
+      Simulation.all_steps_ok tm conf n ->
       Simulation.rules_fit tm ->
       Simulation.decode_state tm
         (Simulation.thiele_step_n_tm tm interpreter_prog
@@ -96,19 +87,19 @@ Definition thiele_universal_witness : interpreter_witness.
 Proof.
   refine {| interpreter_prog := thiele_program;
             interpreter_blind := cpu_program_is_blind |}.
-  intros tm conf n Hok Hfit.
+  intros tm conf n Hall Hfit.
   apply thiele_prefix_simulation_summary; assumption.
 Defined.
 
 Corollary thiele_machine_subsumes_tm :
   forall tm conf n,
-    Simulation.config_ok tm conf ->
+    Simulation.all_steps_ok tm conf n ->
     Simulation.rules_fit tm ->
     Simulation.decode_state tm
       (Simulation.thiele_step_n_tm tm thiele_universal_witness.(interpreter_prog)
          (Simulation.encode_config tm conf) n)
     = TU.tm_step_n tm conf n.
 Proof.
-  intros tm conf n Hok Hfit.
+  intros tm conf n Hall Hfit.
   apply thiele_universal_witness.(interpreter_exact); assumption.
 Qed.
